some seq facts

src/lib/kuiper/Kuiper.Seq.Common.fst
@@ -2,12 +2,32 @@ module Kuiper.Seq.Common
 
 open FStar.Seq
 
-let lemma_seq_fold_left_sum (#a:Type) (e:a) (f: a -> a -> a)
+let lemma_seq_fold_monoid
+  (#a:Type) (e:a) (f: a -> a -> a)
+  (s : seq a)
+  : Lemma (requires is_monoid e f)
+          (ensures seq_fold_left f e s == seq_fold_right f s e)
+  = admit()
+
+let lemma_seq_fold_right_sum
+  (#a:Type) (e:a) (f: a -> a -> a)
+  (s1 s2 : seq a)
+  : Lemma (requires is_monoid e f)
+          (ensures seq_fold_right f (append s1 s2) e
+                   == seq_fold_right f s1 e `f` seq_fold_right f s2 e)
+  = admit()
+
+let lemma_seq_fold_left_sum
+  (#a:Type) (e:a) (f: a -> a -> a)
   (s1 s2 : seq a)
   : Lemma (requires is_monoid e f)
           (ensures seq_fold_left f e (append s1 s2)
-                   == f (seq_fold_left f e s1) (seq_fold_left f e s2))
-  = admit() (* boring *)
+                   == seq_fold_left f e s1 `f` seq_fold_left f e s2)
+  = lemma_seq_fold_monoid e f s1;
+    lemma_seq_fold_monoid e f s2;
+    lemma_seq_fold_monoid e f (append s1 s2);
+    lemma_seq_fold_right_sum e f s1 s2;
+    ()
 
 let lem_append_slice (#a:Type) (s : seq a) (i j k : nat)
   : Lemma (requires i <= j /\ j <= k /\ k <= length s)
